lambda2Gmu/Progress.v
@@ -67,7 +67,8 @@ Theorem progress_thm : progress.
           forwards* [Hv2 | [e2' Hred2]]: IHe2
         ]; clear TypGen EQ T; try rename T2 into T.
   - empty_binding.
-  - admit.
+  - repeat generalize_typings.
+    forwards * [Hval | [? ?]]: IHe.
   - generalize_typings.
     forwards * [Hval | [? ?]]: IHe.
     lets [T' [Typ2 EQ]]: inversion_typing_eq H0.
@@ -80,99 +81,54 @@ Theorem progress_thm : progress.
     apply empty_eq_is_equivalent in EQ. subst.
     lets* [v1 [v2 ?]]: CanonicalFormTuple Typ2; subst.
     right*.
-  - 
-  (* -  *)
-  (*   + apply~ IHe. *)
-
-  (*   IHT e. *)
-  (*   destruct IHt as [ | Hred]. *)
-  (*   + left*. *)
-  (*   + right. *)
-  (*     destruct Hred as [e' Hred]. *)
-  (*     eexists. constructor*. *)
-  (* - left*. *)
-  (* - IHT e1; IHT e2. *)
-  (*   destruct IHt as [IHv1 | IHev1]. *)
-  (*   + destruct IHt0 as [IHv2 | IHev2]. *)
-  (*     * left*. *)
-  (*     * inversion IHev2 as [e2' Hev2]. *)
-  (*       right*. *)
-  (*   + inversion IHev1; right; eauto. *)
-  (* - IHT e. *)
-  (*   destruct IHt as [Hv | Hev]. *)
-  (*   + copy Hv. *)
-  (*     eapply CanonicalFormTuple in Hv; eauto. *)
-  (*     inversion Hv as [v1 Hv2]; inversion Hv2 as [v2 Heq]; subst. *)
-  (*     right*. *)
-
-  (*   + inversion Hev as [e' ev]; eauto. *)
-  (* - IHT e. *)
-  (*   destruct IHt as [Hv | Hev]. *)
-  (*   + copy Hv. *)
-  (*     eapply CanonicalFormTuple in Hv; eauto. *)
-  (*     inversion Hv as [v1 Hv2]; inversion Hv2 as [v2 Heq]; subst. *)
-  (*     right*. *)
-  (*   + inversion Hev as [e' ev]; eauto. *)
-  (* - left; econstructor; econstructor; eauto. *)
-  (* - IHT e1; IHT e2. *)
-  (*   destruct IHt as [Hv1 | Hev1]. *)
-  (*   + destruct IHt0 as [Hv2 | Hev2]. *)
-  (*     * copy Hv1. *)
-  (*       eapply CanonicalFormAbs in Hv1; eauto. *)
-  (*       inversion Hv1 as [v1 Heq]; subst. *)
-  (*       right; eexists; econstructor; eauto. *)
-  (*     * right; inversion Hev2; eexists; eauto. *)
-  (*   + right; inversion Hev1; eexists; eauto. *)
-  (* - left; econstructor; econstructor; eauto. *)
-  (* - IHT e. *)
-  (*   destruct IHt as [Hv | Hev]. *)
-  (*   + right. *)
-  (*     eapply CanonicalFormTAbs in Hv; eauto. *)
-  (*     inversion Hv as [v1 eq]; subst. *)
-  (*     eexists. econstructor; eauto. *)
-  (*   + right; inversion Hev; eauto. *)
-  (* - right. *)
-  (*   eexists. *)
-  (*   constructor*. *)
-  (* - right. *)
-  (*   rename l into ms. *)
-  (*   inversions Htyp. *)
-  (*   lets* IHe2: IHe H2. *)
-  (*   destruct IHe2 as [Hval | [e' Hred]]. *)
-  (*   + lets* [GCargs [GCind [GCterm Heq]]]: CanonicalFormGadt H2. *)
-  (*     subst. *)
-
-  (*     match goal with *)
-  (*     | [ H: {?A, ?B, ?C} ⊢ trm_constructor ?D ?E ?F ∈ ?G |- _ ] => *)
-  (*       inversions H *)
-  (*     end. *)
-  (*     lets* bindeq: binds_ext H4 H6. *)
-  (*     inversions bindeq. *)
-  (*     lets* bindeq: binds_ext H4 H9. *)
-  (*     inversions bindeq. *)
-
-  (*     lets: nth_error_implies_zip. *)
-  (*     match goal with *)
-  (*     | [ Hnth: List.nth_error ?As ?i = Some ?A |- _ ] => *)
-  (*       match goal with *)
-  (*       | [ Hlen: length As = length ?Bs |- _ ] => *)
-  (*         lets* [[clA clT] [nth_cl inzip]]: nth_error_implies_zip Hnth Hlen *)
-  (*       end *)
-  (*     end. *)
-  (*     assert (clA = length GCargs). *)
-  (*     * match goal with *)
-  (*       | [ H: forall def clause, List.In (def, clause) ?A -> clauseArity clause = Carity def |- _ ] => *)
-  (*         lets*: H inzip *)
-  (*       end. *)
-  (*     * subst. *)
-  (*       eexists. *)
-  (*       econstructor; eauto. *)
-  (*   + eexists; eauto. *)
-  (* - IHT e1. *)
-  (*   right. destruct IHt as [Hv | Hev]. *)
-  (*   + eexists. econstructor; eauto. *)
-  (*   + inversion Hev as [e1' ev]. *)
-  (*     eexists; eapply ered_let; eauto. *)
-
-  (* - eapply typing_implies_term; eauto. *)
-Admitted.
+  - repeat generalize_typings.
+    forwards * [Hval1 | [? ?]]: IHe1.
+    forwards * [Hval2 | [? ?]]: IHe2.
+    right.
+    lets [T' [Typ2 EQ]]: inversion_typing_eq H5.
+    apply empty_eq_is_equivalent in EQ. subst.
+    lets* [v1 ?]: CanonicalFormAbs Typ2; subst.
+    eexists.
+    apply* red_beta.
+  - repeat generalize_typings.
+    forwards * [Hval1 | [? ?]]: IHe.
+    right.
+    lets [T' [Typ2 EQ]]: inversion_typing_eq H1.
+    apply empty_eq_is_equivalent in EQ. subst.
+    lets* [v1 ?]: CanonicalFormTAbs Typ2; subst.
+    eexists.
+    apply* red_tbeta.
+  - repeat generalize_typings.
+    right.
+    eexists.
+    eauto.
+  - right.
+    rename l into branches.
+    repeat generalize_typings.
+    forwards * [Hval1 | [? ?]]: IHe.
+    lets [T' [Typ2 EQ]]: inversion_typing_eq H2.
+    apply empty_eq_is_equivalent in EQ; subst.
+    lets* [GCargs [cid [ctor_e ?]]]: CanonicalFormGadt Typ2; subst.
+    inversions Typ2.
+    match goal with
+    | [ H1: binds ?g ?A Σ, H2: binds ?g ?B Σ |- _ ] =>
+      let H := fresh "H" in
+      lets H: binds_ext H1 H2;
+        inversions H
+    end.
+    match goal with
+    | [ Hnth: List.nth_error ?As ?i = Some ?A |- _ ] =>
+      match goal with
+      | [ Hlen: length As = length ?Bs |- _ ] =>
+        lets* [[clA clT] [nth_cl inzip]]: nth_error_implies_zip Hnth Hlen
+      end
+    end.
+    assert (clA = length GCargs).
+    * match goal with
+      | [ H: forall def clause, List.In (def, clause) ?A -> clauseArity clause = Carity def |- _ ] =>
+        lets*: H inzip
+      end.
+    * subst.
+      eexists.
+      eauto.
+Qed.
